src/rocq/Handlers/Memory.v
@@ -14,56 +14,88 @@ From ITree Require Import
   Events.StateFacts
   Basics.MonadState.
 
+Import Basics.Basics.Monads.
+
 From Vellvm Require Import
   Utilities
   Syntax
   Params
   Semantics.LLVMEvents
   Semantics.DynamicValues
-  Semantics.Memory.
+  Semantics.Params.Memory
+  Semantics.Params.VellvmImplem.Memory.
 
 From QuickChick Require Import Show.
 
 
 Section withParams.
   Context {Pa : Params}.
-
+  Context  {E} `{FailureE -< E} `{UBE -< E} `{OOME -< E}.
   Existing Instance MemoryModelPrimitivesV.
   
-  Definition handle_memory {E} (h : memM ~> itree E) : MemoryE ~> itree E :=
+  Definition handle_memory {E} (h : memM ~> stateT state (itree E))
+    : MemoryE ~> stateT state (itree E) :=
     fun T e => h _ (handle_memoryM e).
 
-  (* Hmmm may have made a mistake somewhere: how do I access the current state?
-     It is stored in the event, but not at the top level... *)
-  Fixpoint memM_interp {E}
-    `{FailureE -< E}
-    `{UBE -< E}
-    `{OOME -< E}
-    : memM ~> itree E.
-    refine (fun T m => match m with
-                    | Mret x => ret x
-                    | Moom s => raiseOOM s
-                    | Mub s => raiseUB s
-                    | Merr s => raise s
-                    | Mfresh_addr σ k => _
-                    | Mfresh_prov σ k => _
-                    end
-           ).
-      
-  Definition mem_state_fresh_provenance (ms : state) : (Provenance * state) :=
-    match ms with
-    | mkMemState mem_stack pr =>
-        let pr' := next_provenance pr in
-        (pr', mkMemState mem_stack pr')
-    end.
+  Definition fresh_provenance : stateT state (itree E) provenance :=
+    fun σ => let p' := next_provenance σ.(state_provenance) in
+          ret ({| state_memory_stack := σ.(state_memory_stack) ;
+                 state_provenance := p' |} ,p').
+ 
+  Fixpoint memM_interp
+    : memM ~> stateT state (itree E) :=
+    fun T m σ => match m with
+              | Mret x => ret (σ, x)
+              | Moom s => raiseOOM s
+              | Mub s => raiseUB s
+              | Merr s => raise s
+              | Mget   k => memM_interp (k σ) σ
+              | Mput σ' k => memM_interp k σ'
+              | Mnext_key k => memM_interp (k (IntMaps.next_key σ.(state_memory_stack).(Memory_stack_memory))) σ
+              | Mfresh_prov k => '(σ',p) <- fresh_provenance σ ;; memM_interp (k p) σ'
+              end
+  .
 
-
-  Definition memM_model {E} : memM ~> itree E.
-    intros T e.
-    induction e.
-  
+(* TODO: Same signature for the model,
+   but branching based on ctrees instead. *)
+  (*   Fixpoint memM_model *)
+  (*   : memM ~> stateT state (itree E). *)
+  (*   fun T m σ => match m with *)
+  (*             | Mret x => ret (σ, x) *)
+  (*             | Moom s => raiseOOM s *)
+  (*             | Mub s => raiseUB s *)
+  (*             | Merr s => raise s *)
+  (*             | Mget   k => memM_interp (k σ) σ *)
+  (*             | Mput σ' k => memM_interp k σ' *)
+  (*             | Mnext_key k =>  *)
+  (*             | Mfresh_prov k => *)
+  (*             end *)
+  (* . *)
+ 
 End withParams.
 
+Section PARAMS.
+  Context {Pa : Params}.
+  Existing Instance MemoryModelPrimitivesV.
+  
+  Variable (E F G: Type -> Type).
+  Context  `{FailureE -< G} `{UBE -< G} `{OOME -< G}.
+  Notation Effin := (E +' F +' MemoryE +' G).
+  Notation Effout := (E +' F +' G).
 
+  Definition E_trigger {M} : forall R, E R -> (stateT M (itree Effout) R) :=
+    fun R e m => r <- trigger e ;; ret (m, r).
 
+  Definition F_trigger {M} : forall R, F R -> (stateT M (itree Effout) R) :=
+    fun R e m => r <- trigger e ;; ret (m, r).
 
+  Definition G_trigger {M} : forall R, G R -> (stateT M (itree Effout) R) :=
+    fun R e m => r <- trigger e ;; ret (m, r).
+  
+  Definition interp_memory_h : Effin ~> stateT state (itree Effout) :=
+    case_ E_trigger (case_ F_trigger (case_ (handle_memory memM_interp) G_trigger)).
+  
+  Definition interp_memory : itree Effin ~> stateT state (itree Effout) :=
+    interp_state interp_memory_h.
+
+End PARAMS.
